Elpi Run -> Elpi Query

theories/test_param.v
@@ -10,7 +10,7 @@ Class param {X : Type} {XR : X -> X -> Type} (x : X) (xR : XR x x) := Param {}.
 Elpi Tactic param " typecheck.".
 Elpi Accumulate File "coq-extra.elpi".
 Elpi Accumulate File "coq-param.elpi".
-Elpi Run param "typecheck".
+Elpi Query param "typecheck".
 
 Elpi Print param "param.html"
   "pervasives.elpi"
@@ -18,77 +18,77 @@ Elpi Print param "param.html"
   "lp-lib.elpi"
   "coq-refiner.elpi".
 
-Elpi Run param "env-add-param {{@unit}} ""unitR""".
-Elpi Run param "env-add-param {{@nat}} ""natR""".
+Elpi Query param "env-add-param {{@unit}} ""unitR""".
+Elpi Query param "env-add-param {{@nat}} ""natR""".
 
 Inductive fin : nat -> Type :=
     FO : fin 0 | FS : forall n : nat, fin n -> fin (S n).
-Elpi Run param "env-add-param {{@fin}} ""finR"")".
+Elpi Query param "env-add-param {{@fin}} ""finR"")".
 
 Fixpoint fin_length  n (v : fin n) :=
   match v with FO => 0 | FS _ w => S (fin_length _ w) end.
-Elpi Run param "env-add-param {{@fin_length}} ""fin_lengthR"")".
+Elpi Query param "env-add-param {{@fin_length}} ""fin_lengthR"")".
 
 Inductive vec (A : Type) : nat -> Type :=
     nil : vec A 0 | cons : A -> forall n : nat, vec A n -> vec A (S n).
-Elpi Run param "env-add-param {{@vec}} ""vecR"")".
+Elpi Query param "env-add-param {{@vec}} ""vecR"")".
 
 Fixpoint vec_length (A : Type) n (v : vec A n) :=
   match v with nil _ => 0 | cons _ _ _ w => S (vec_length _ _ w) end.
-Elpi Run param "env-add-param {{@vec_length}} ""vec_lengthR"")".
+Elpi Query param "env-add-param {{@vec_length}} ""vec_lengthR"")".
 
 
-Elpi Run param "env-add-param {{@list}} ""listR""".
-Elpi Run param "env-add-param {{@eq}} ""eqR""".
+Elpi Query param "env-add-param {{@list}} ""listR""".
+Elpi Query param "env-add-param {{@eq}} ""eqR""".
 
 Fixpoint plus' m n := match n with 0 => m | S n => S (plus' m n) end.
-Elpi Run param "env-add-param {{@plus'}} ""plus'R""".
-Elpi Run param "env-add-param {{@plus}} ""plusR""".
+Elpi Query param "env-add-param {{@plus'}} ""plus'R""".
+Elpi Query param "env-add-param {{@plus}} ""plusR""".
 
 Definition test m n p q r := m + n + p + q + r.
-Elpi Run param "env-add-param {{@test}} ""testR""".
+Elpi Query param "env-add-param {{@test}} ""testR""".
 
 Definition vec_length_type := forall (A : Type) (n : nat), vec A n -> nat.
 
-Elpi Run param "env-add-param {{@vec_length_type}} ""vec_length_typeR"")".
+Elpi Query param "env-add-param {{@vec_length_type}} ""vec_length_typeR"")".
 
 Definition vec_length_rec (vec_length : vec_length_type)
   (A : Type) n (v : vec A n) :=
   match v with nil _ => 0 | cons _ _ _ w => S (vec_length _ _ w) end.
-Elpi Run param "env-add-param {{@vec_length_rec}} ""vec_length_recR"")".
+Elpi Query param "env-add-param {{@vec_length_rec}} ""vec_length_recR"")".
 
-Elpi Run param "with-TC-param (param {{O}} X Y)".
-Elpi Run param "with-TC-param (param {{S (S 0)}} X Y)".
+Elpi Query param "with-TC-param (param {{O}} X Y)".
+Elpi Query param "with-TC-param (param {{S (S 0)}} X Y)".
 
-Fail Elpi Run param "param-const {{@eq_refl}} _ _ _ _ _ _".
+Fail Elpi Query param "param-const {{@eq_refl}} _ _ _ _ _ _".
 
-Elpi Run param "with-TC {{@param_db}} retrieve-param (param {{nat}} X Y)".
+Elpi Query param "with-TC {{@param_db}} retrieve-param (param {{nat}} X Y)".
 
 Definition nat2nat := nat -> nat.
 Definition nat2nat2nat := nat -> nat -> nat.
-Elpi Run param "env-add-param {{@nat2nat}} ""nat2natR""".
-Elpi Run param "env-add-param {{@nat2nat2nat}} ""nat2nat2natR""".
-Elpi Run param "env-add-param {{@pred}} ""predR""".
+Elpi Query param "env-add-param {{@nat2nat}} ""nat2natR""".
+Elpi Query param "env-add-param {{@nat2nat2nat}} ""nat2nat2natR""".
+Elpi Query param "env-add-param {{@pred}} ""predR""".
 Print predR.
 Check (predR : nat2natR pred pred).
 
 Fixpoint predn n := match n with 0 => 0 | S n => S (predn n) end.
 
-Elpi Run param "env-add-param {{@predn}} ""prednR""".
+Elpi Query param "env-add-param {{@predn}} ""prednR""".
 
 Check (prednR : nat2natR predn predn).
 Check (plusR : nat2nat2natR plus plus).
 
 Fixpoint quasidn n m := S (match n with 0 => m | S n => S (quasidn n m) end).
-Elpi Run param "param-const {{@quasidn}} _ _ _ _ XR _".
+Elpi Query param "param-const {{@quasidn}} _ _ _ _ XR _".
 
 Fixpoint weirdn n := match n with S (S n) => S (weirdn n) | _ => 0 end.
-Elpi Run param "param-const {{@weirdn}} _ _ _ _ XR _".
+Elpi Query param "param-const {{@weirdn}} _ _ _ _ XR _".
 
 Inductive bla : nat -> Type := Bla : nat -> bla 0 | Blu n : bla n -> bla 1.
-Elpi Run param "env-add-param {{@bla}} ""blaR"")".
+Elpi Query param "env-add-param {{@bla}} ""blaR"")".
 
-Elpi Run param "coq-TC-db-for {term->gr {{@param_db}}} PDb".
+Elpi Query param "coq-TC-db-for {term->gr {{@param_db}}} PDb".
 
 
 Fixpoint silly (n : nat) := n.
